\section{Problem 3}
\begin{align*}
1-g(x) = 1 - \cfrac{1}{1+\cfrac{1}{{e^x}}} \Leftrightarrow 
1-g(x) = 1 - \cfrac{1}{\cfrac{e^x + 1}{e^x}} \Leftrightarrow \\
1-g(x) = 1 - \cfrac{e^x}{e^x + 1} \Leftrightarrow 
1-g(x) = \cfrac{e^x+1-e^x}{e^x+1} \Leftrightarrow \\
1-g(x) = \cfrac{1}{e^x+1} \Leftrightarrow 
1-g(x) = g(-x)
\end{align*}
\begin{align*}
g(x) = \frac{1}{1+e^{-x}} = y \\
y+y*e^{-x} = 1 \Rightarrow 
e^{-x} = \frac{1-y}{y} \Rightarrow \\
e^x = \frac{y}{1-y} \Rightarrow 
\ln(e^x) = \ln(\frac{y}{1-y}) \Rightarrow \\
x = \ln(\frac{y}{1-y}) \Rightarrow 
g(y) = \ln(\frac{y}{1-y})
\end{align*}
